src/program_proof/mvcc/examples_counter.v
@@ -1,0 +1,386 @@
+From iris.base_logic Require Import mono_nat.
+(* This should go first otherwise the default scope becomes nat. *)
+From Perennial.program_proof Require Import grove_prelude.
+From Goose.github_com.mit_pdos.go_mvcc Require Import examples.
+From Perennial.program_proof.mvcc Require Import txn_proof.
+
+Section program.
+Context `{!heapGS Σ, !mvcc_ghostG Σ, !mono_natG Σ}.
+
+#[local]
+Definition mvcc_inv_app_def γ α : iProp Σ :=
+  ∃ (v : u64),
+    "Hdbpt" ∷ dbmap_ptsto γ (U64 0) 1 (Value v) ∗
+    "Hmn"   ∷ mono_nat_auth_own α 1 (int.nat v).
+
+Instance mvcc_inv_app_timeless γ α :
+  Timeless (mvcc_inv_app_def γ α).
+Proof. unfold mvcc_inv_app_def. apply _. Defined.
+
+#[local]
+Definition mvccNApp := nroot .@ "app".
+#[local]
+Definition mvcc_inv_app γ α : iProp Σ :=
+  inv mvccNApp (mvcc_inv_app_def γ α).
+
+Definition P_Increment (r : dbmap) := ∃ v, r = {[ (U64 0) := (Value v) ]}.
+Definition Q_Increment (r w : dbmap) :=
+  ∃ (v u : u64),
+    r !! (U64 0) = Some (Value v) ∧
+    w !! (U64 0) = Some (Value u) ∧
+    int.Z u = int.Z v + 1.
+
+(**
+ * [p] is not used until [R/R1/R2] are added to [wp_txn__DoTxn].
+ *)
+Theorem wp_IncrementSeq txn (p : loc) tid r γ τ :
+  {{{ own_txn txn tid r γ τ ∗ ⌜P_Increment r⌝ ∗ txnmap_ptstos τ r }}}
+    IncrementSeq #txn #p
+  {{{ (ok : bool), RET #ok;
+      own_txn txn tid r γ τ ∗
+      if ok then ∃ w, ⌜Q_Increment r w ∧ dom r = dom w⌝ ∗ txnmap_ptstos τ w else True
+  }}}.
+Proof.
+  iIntros (Φ) "(Htxn & %HP & Hpt) HΦ".
+  wp_call.
+
+  (***********************************************************)
+  (* v, _ := txn.Get(0)                                      *) 
+  (***********************************************************)
+  destruct HP as [v Hr].
+  unfold txnmap_ptstos.
+  rewrite {2} Hr.
+  rewrite big_sepM_singleton.
+  wp_apply (wp_txn__Get with "[$Htxn $Hpt]").
+  iIntros (v' found).
+  iIntros "(Htxn & Hpt & %Hv)".
+  (* From the precondition we know [found] can only be [true]. *)
+  unfold to_dbval in Hv. destruct found; last done.
+  inversion Hv.
+  subst v'.
+  wp_pures.
+
+  (***********************************************************)
+  (* if v == 18446744073709551615 {                          *) 
+  (*     return false                                        *) 
+  (* }                                                       *) 
+  (***********************************************************)
+  wp_if_destruct.
+  { iApply "HΦ". by iFrame. }
+
+  (***********************************************************)
+  (* txn.Put(0, v + 1)                                       *)
+  (***********************************************************)
+  wp_apply (wp_txn__Put with "[$Htxn $Hpt]").
+  iIntros "[Htxn Hpt]".
+  wp_pures.
+
+  (***********************************************************)
+  (* return true                                             *)
+  (***********************************************************)
+  iApply "HΦ".
+  rewrite -big_sepM_singleton.
+  iFrame "Htxn".
+  iExists _. iFrame "Hpt".
+  iPureIntro.
+  split; last set_solver.
+  unfold Q_Increment.
+  eexists _, _.
+  split.
+  { rewrite Hr. by rewrite lookup_singleton. }
+  split.
+  { by rewrite lookup_singleton. }
+  apply u64_val_ne in Heqb.
+  word.
+Qed.
+
+Theorem wp_Increment (txn : loc) (p : loc) γ :
+  ⊢ {{{ own_txn_uninit txn γ }}}
+    <<< ∀∀ (r : dbmap), ⌜P_Increment r⌝ ∗ dbmap_ptstos γ 1 r >>>
+      Increment #txn #p @ ↑mvccNSST
+    <<< ∃∃ (ok : bool), if ok then (∃ w, ⌜Q_Increment r w⌝ ∗ dbmap_ptstos γ 1 w) else dbmap_ptstos γ 1 r >>>
+    {{{ RET #ok; own_txn_uninit txn γ }}}.
+Proof.
+  iIntros "!>".
+  iIntros (Φ) "Htxn HAU".
+  wp_call.
+
+  (***********************************************************)
+  (* body := func(txn *txn.Txn) bool {                       *) 
+  (*     return DecrementSeq(txn, p)                         *) 
+  (* }                                                       *) 
+  (* return t.DoTxn(body)                                    *) 
+  (***********************************************************)
+  wp_apply (wp_txn__DoTxn _ _ _ Q_Increment with "[$Htxn]").
+  { unfold spec_body.
+    iIntros (tid r τ Φ') "!> HP HΦ'".
+    wp_pures.
+    iApply (wp_IncrementSeq with "HP HΦ'").
+  }
+  done.
+Qed.
+
+Definition P_Decrement (r : dbmap) := ∃ v, r = {[ (U64 0) := (Value v) ]}.
+Definition Q_Decrement (r w : dbmap) :=
+  ∃ (v u : u64),
+    r !! (U64 0) = Some (Value v) ∧
+    w !! (U64 0) = Some (Value u) ∧
+    int.Z u = int.Z v - 1.
+
+(**
+ * [p] is not used until [R/R1/R2] are added to [wp_txn__DoTxn].
+ *)
+Theorem wp_DecrementSeq txn (p : loc) tid r γ τ :
+  {{{ own_txn txn tid r γ τ ∗ ⌜P_Decrement r⌝ ∗ txnmap_ptstos τ r }}}
+    DecrementSeq #txn #p
+  {{{ (ok : bool), RET #ok;
+      own_txn txn tid r γ τ ∗
+      if ok then ∃ w, ⌜Q_Decrement r w ∧ dom r = dom w⌝ ∗ txnmap_ptstos τ w else True
+  }}}.
+Proof.
+  iIntros (Φ) "(Htxn & %HP & Hpt) HΦ".
+  wp_call.
+
+  (***********************************************************)
+  (* v, _ := txn.Get(0)                                      *) 
+  (***********************************************************)
+  destruct HP as [v Hr].
+  unfold txnmap_ptstos.
+  rewrite {2} Hr.
+  rewrite big_sepM_singleton.
+  wp_apply (wp_txn__Get with "[$Htxn $Hpt]").
+  iIntros (v' found).
+  iIntros "(Htxn & Hpt & %Hv)".
+  (* From the precondition we know [found] can only be [true]. *)
+  unfold to_dbval in Hv. destruct found; last done.
+  inversion Hv.
+  subst v'.
+  wp_pures.
+
+  (***********************************************************)
+  (* if v == 0 {                                             *) 
+  (*     return false                                        *) 
+  (* }                                                       *) 
+  (***********************************************************)
+  wp_if_destruct.
+  { iApply "HΦ". by iFrame. }
+
+  (***********************************************************)
+  (* txn.Put(0, v + 1)                                       *)
+  (***********************************************************)
+  wp_apply (wp_txn__Put with "[$Htxn $Hpt]").
+  iIntros "[Htxn Hpt]".
+  wp_pures.
+
+  (***********************************************************)
+  (* return true                                             *)
+  (***********************************************************)
+  iApply "HΦ".
+  rewrite -big_sepM_singleton.
+  iFrame "Htxn".
+  iExists _. iFrame "Hpt".
+  iPureIntro.
+  split; last set_solver.
+  unfold Q_Decrement.
+  eexists _, _.
+  split.
+  { rewrite Hr. by rewrite lookup_singleton. }
+  split.
+  { by rewrite lookup_singleton. }
+  apply u64_val_ne in Heqb.
+  replace (int.Z 0) with 0 in Heqb by word.
+  word.
+Qed.
+
+Theorem wp_Decrement (txn : loc) (p : loc) γ :
+  ⊢ {{{ own_txn_uninit txn γ }}}
+    <<< ∀∀ (r : dbmap), ⌜P_Decrement r⌝ ∗ dbmap_ptstos γ 1 r >>>
+      Decrement #txn #p @ ↑mvccNSST
+    <<< ∃∃ (ok : bool), if ok then (∃ w, ⌜Q_Decrement r w⌝ ∗ dbmap_ptstos γ 1 w) else dbmap_ptstos γ 1 r >>>
+    {{{ RET #ok; own_txn_uninit txn γ }}}.
+Proof.
+  iIntros "!>".
+  iIntros (Φ) "Htxn HAU".
+  wp_call.
+
+  (***********************************************************)
+  (* body := func(txn *txn.Txn) bool {                       *) 
+  (*     return DecrementSeq(txn, p)                         *) 
+  (* }                                                       *) 
+  (* return t.DoTxn(body)                                    *) 
+  (***********************************************************)
+  wp_apply (wp_txn__DoTxn _ _ _ Q_Decrement with "[$Htxn]").
+  { unfold spec_body.
+    iIntros (tid r τ Φ') "!> HP HΦ'".
+    wp_pures.
+    iApply (wp_DecrementSeq with "HP HΦ'").
+  }
+  done.
+Qed.
+
+(*****************************************************************)
+(* func InitializeData(txnmgr *txn.TxnMgr)                       *)
+(*****************************************************************)
+Theorem wp_InitializeData (txnmgr : loc) γ :
+  is_txnmgr txnmgr γ -∗
+  {{{ dbmap_ptstos γ 1 (gset_to_gmap Nil keys_all) }}}
+    InitializeData #txnmgr
+  {{{ α, RET #(); mvcc_inv_app γ α }}}.
+Proof.
+Admitted.
+
+Theorem wp_InitExample :
+  {{{ True }}}
+    InitExample #()
+  {{{ γ α (mgr : loc), RET #mgr; is_txnmgr mgr γ ∗ mvcc_inv_app γ α }}}.
+Proof.
+  iIntros (Φ) "_ HΦ".
+  wp_call.
+
+  (***********************************************************)
+  (* mgr := txn.MkTxnMgr()                                   *)
+  (* InitializeData(mgr)                                     *)
+  (* return mgr                                              *)
+  (***********************************************************)
+  wp_apply wp_MkTxnMgr.
+  iIntros (γ mgr) "[#Hmgr Hdbpts]".
+  wp_pures.
+  wp_apply (wp_InitializeData with "Hmgr [$Hdbpts]").
+  iIntros (α) "#Hinv".
+  wp_pures.
+  iModIntro.
+  iApply "HΦ".
+  iFrame "∗ #".
+Qed.
+
+Theorem wp_CallIncrement (mgr : loc) γ α :
+  mvcc_inv_app γ α -∗
+  is_txnmgr mgr γ -∗
+  {{{ True }}}
+    CallIncrement #mgr
+  (* TODO: give lower bound of the counter. *)
+  {{{ (v : u64) (ok : bool), RET (#v, #ok); True }}}.
+Proof.
+  iIntros "#Hinv #Hmgr" (Φ) "!> _ HΦ".
+  wp_call.
+
+  (***********************************************************)
+  (* txn := mgr.New()                                        *)
+  (***********************************************************)
+  wp_apply (wp_txnMgr__New with "Hmgr").
+  iNamed "Hmgr".
+  iIntros (txn) "Htxn".
+  wp_pures.
+
+  (***********************************************************)
+  (* var n uint64                                            *)
+  (* ok := Increment(txn, &n)                                *)
+  (***********************************************************)
+  wp_apply wp_ref_of_zero; first done.
+  iIntros (vRef) "HvRef".
+  wp_pures.
+  wp_apply (wp_Increment with "Htxn").
+  iInv "Hinv" as "> HinvO" "HinvC".
+  iApply ncfupd_mask_intro; first set_solver.
+  iIntros "Hclose".
+  iNamed "HinvO".
+  (* Give atomic precondition. *)
+  iExists {[ (U64 0) := (Some v) ]}.
+  unfold dbmap_ptstos. rewrite {1} big_sepM_singleton.
+  iFrame.
+  iSplit.
+  { iPureIntro. unfold P_Increment. by eauto. }
+  (* Take atomic postcondition. *)
+  iIntros (ok) "H".
+  iMod "Hclose" as "_".
+
+  (***********************************************************)
+  (* return v, ok                                            *)
+  (***********************************************************)
+  destruct ok eqn:E.
+  { (* Case COMMIT. *)
+    iDestruct "H" as (w) "[%HQ Hdbpt]".
+    unfold Q_Increment in HQ.
+    destruct HQ as (v' & u' & Hlookupr & Hlookupw & Hvu).
+    (* Show [v = v']. *)
+    rewrite lookup_singleton in Hlookupr. inversion_clear Hlookupr.
+    iDestruct (big_sepM_lookup with "Hdbpt") as "Hdbpt"; first apply Hlookupw.
+    iMod (mono_nat_own_update (int.nat u') with "Hmn") as "[Hmn #Hmnlb]".
+    { (* Show [int.nat v' ≤ int.nat u']. *) word. }
+    iMod ("HinvC" with "[- HΦ HvRef]") as "_".
+    { (* Close the invariant. *) iExists _. iFrame. }
+    iIntros "!> Htxn".
+    wp_load.
+    wp_pures.
+    iApply "HΦ".
+    by iFrame.
+  }
+  { (* Case ABORT. *)
+    unfold dbmap_ptstos. rewrite big_sepM_singleton.
+    iMod ("HinvC" with "[- HΦ HvRef]") as "_".
+    { (* Close the invariant. *) iExists _. iFrame. }
+    iIntros "!> Htxn".
+    wp_load.
+    wp_pures.
+    iApply "HΦ".
+    by iFrame.
+  }
+Qed.
+
+Theorem wp_CallDecrement (mgr : loc) γ α :
+  mvcc_inv_app γ α -∗
+  is_txnmgr mgr γ -∗
+  {{{ True }}}
+    CallDecrement #mgr
+  {{{ (v : u64) (ok : bool), RET (#v, #ok); True }}}.
+Proof.
+  iIntros "#Hinv #Hmgr" (Φ) "!> _ HΦ".
+  wp_call.
+
+  (***********************************************************)
+  (* txn := mgr.New()                                        *)
+  (***********************************************************)
+  wp_apply (wp_txnMgr__New with "Hmgr").
+  iNamed "Hmgr".
+  iIntros (txn) "Htxn".
+  wp_pures.
+
+  (***********************************************************)
+  (* var n uint64                                            *)
+  (* ok := Decrement(txn, &n)                                *)
+  (***********************************************************)
+  wp_apply wp_ref_of_zero; first done.
+  iIntros (vRef) "HvRef".
+  wp_pures.
+  wp_apply (wp_Decrement with "Htxn").
+  iInv "Hinv" as "> HinvO" "HinvC".
+  iApply ncfupd_mask_intro; first set_solver.
+  iIntros "Hclose".
+  iNamed "HinvO".
+  (* Give atomic precondition. *)
+  iExists {[ (U64 0) := (Some v) ]}.
+  unfold dbmap_ptstos. rewrite {1} big_sepM_singleton.
+  iFrame.
+  iSplit.
+  { iPureIntro. unfold P_Decrement. by eauto. }
+  (* Take atomic postcondition. *)
+  iIntros (ok) "H".
+  iMod "Hclose" as "_".
+
+  (***********************************************************)
+  (* return n, ok                                            *)
+  (***********************************************************)
+  destruct ok eqn:E.
+  { (* Case COMMIT. *)
+    iDestruct "H" as (w) "[%HQ Hdbpt]".
+    unfold Q_Increment in HQ.
+    destruct HQ as (v' & u' & Hlookupr & Hlookupw & Hvu).
+    (* Show [v = v']. *)
+    rewrite lookup_singleton in Hlookupr. inversion_clear Hlookupr.
+    iDestruct (big_sepM_lookup with "Hdbpt") as "Hdbpt"; first apply Hlookupw.
+    iMod (mono_nat_own_update (int.nat u') with "Hmn") as "[Hmn #Hmnlb]".
+    { (* Cannot show [int.nat v' ≤ int.nat u']. *)
+      Fail word.
+Abort.
+
+End program.
